Kura/Operation/Minor2Simp.lean
@@ -7,18 +7,20 @@ variable {α β α' α'' β' : Type*} {u v w x y z : Set α} {e f : Sym2 (Set α
 
 namespace Graph
 
-@[simps!?]
+@[simps!]
 def SimpMinor (G : Graph (Set α) (Sym2 (Set α))) (C : Set (Sym2 (Set α))) : Graph (Set α) (Sym2 (Set α)) :=
   G / C |>.Simplify
+
+scoped infix:50 " // " => Graph.SimpMinor
 
 #print Graph.SimpMinor_inc₂
 
 theorem simpMinor_inc₂ (G : Graph (Set α) (Sym2 (Set α))) (C : Set (Sym2 (Set α))) :
-    (G.SimpMinor C).Inc₂ e x y ↔ (G / C).Adj x y ∧ x ≠ y ∧ e = s(x, y) := by
-  rw [SimpMinor_inc₂, ← and_assoc (b := x ≠ y), and_congr_left_iff]
+    (G // C).Inc₂ e x y ↔ x ≠ y ∧ (G / C).Adj x y  ∧ e = s(x, y) := by
+  rw [SimpMinor_inc₂, ← and_assoc (a := x ≠ y), and_congr_left_iff]
   rintro rfl
   simp only [toSym2_eq_pair_iff, SetContract_inc₂, exists_and_left, exists_prop,
-    Sym2.isDiag_iff_proj_eq, ne_eq, and_congr_left_iff]
+    Sym2.isDiag_iff_proj_eq, ne_eq, and_congr_right_iff]
   rintro hne
   refine ⟨fun ⟨s, hsC, ⟨hs, _⟩, u, v, hbtw, hx, hy⟩ ↦ ?_, fun ⟨e, hbtw⟩ ↦ ?_⟩
   · use s
@@ -31,19 +33,13 @@ theorem simpMinor_inc₂ (G : Graph (Set α) (Sym2 (Set α))) (C : Set (Sym2 (Se
     exact ⟨e, hbtw.1, ⟨this, hbtw.1⟩, hbtw.2⟩
 
 theorem simpMinor_adj (G : Graph (Set α) (Sym2 (Set α))) (C : Set (Sym2 (Set α))) :
-    (G.SimpMinor C).Adj x y ↔ (G / C).Adj x y ∧ x ≠ y := by
+    (G // C).Adj x y ↔ x ≠ y ∧ (G / C).Adj x y := by
   simp_rw [Adj, simpMinor_inc₂, ← and_assoc]
   rw [exists_eq_right, ← Graph.Adj]
 
 instance simpMinor_isSimpleCanonical (G : Graph (Set α) (Sym2 (Set α))) (C : Set (Sym2 (Set α))) :
-    IsSimpleCanonical (G.SimpMinor C) where
-  loopless x := by
-    simp only [simpMinor_adj, ne_eq, not_true_eq_false, and_false, not_false_eq_true]
-  no_multi_edges e f he hf h := by
-    induction' e with u v
-    induction' f with x y
-    simp only [SimpMinor_edgeSet, mem_setOf_eq, toSym2_eq_pair_iff, SetContract_inc₂,
-      exists_and_left, exists_prop, Sym2.isDiag_iff_proj_eq] at he hf
-    obtain ⟨he, he'⟩ := he
+    SimpleCanonical (G // C) := instSimpleCanonicalSimplify
+
+
 
 end Graph
